@prefix : <https://w3id.org/np/o/ntemplate/NanopubTemplateOntology#> .
@prefix owl: <http://www.w3.org/2002/07/owl#> .
@prefix rdf: <http://www.w3.org/1999/02/22-rdf-syntax-ns#> .
@prefix xml: <http://www.w3.org/XML/1998/namespace> .
@prefix xsd: <http://www.w3.org/2001/XMLSchema#> .
@prefix rdfs: <http://www.w3.org/2000/01/rdf-schema#> .
@base <https://w3id.org/np/o/ntemplate/NanopubTemplateOntology> .

<https://w3id.org/np/o/ntemplate/NanopubTemplateOntology> rdf:type owl:Ontology ;
                                                           <http://purl.org/dc/terms/creator> <https://orcid.org/0000-0002-1267-0234> ;
                                                           <http://purl.org/dc/terms/description> "This is an ontology to describe nanopublication templates, which can be published as nanopublications themselves." ;
                                                           <http://purl.org/dc/terms/license> <https://creativecommons.org/publicdomain/zero/1.0/> ;
                                                           <http://purl.org/dc/terms/title> "Nanopublication Template Ontology" ;
                                                           <http://purl.org/vocab/vann/preferredNamespacePrefix> "nt" ;
                                                           <http://purl.org/vocab/vann/preferredNamespaceUri> "https://w3id.org/np/o/ntemplate/" ;
                                                           rdfs:isDefinedBy <https://w3id.org/np/o/ntemplate/latest/NanopubTemplateOntology> .

#################################################################
#    Annotation properties
#################################################################

###  http://purl.org/dc/terms/creator
<http://purl.org/dc/terms/creator> rdf:type owl:AnnotationProperty .


###  http://purl.org/dc/terms/description
<http://purl.org/dc/terms/description> rdf:type owl:AnnotationProperty .


###  http://purl.org/dc/terms/license
<http://purl.org/dc/terms/license> rdf:type owl:AnnotationProperty .


###  http://purl.org/dc/terms/title
<http://purl.org/dc/terms/title> rdf:type owl:AnnotationProperty .


###  http://purl.org/vocab/vann/preferredNamespacePrefix
<http://purl.org/vocab/vann/preferredNamespacePrefix> rdf:type owl:AnnotationProperty .


###  http://purl.org/vocab/vann/preferredNamespaceUri
<http://purl.org/vocab/vann/preferredNamespaceUri> rdf:type owl:AnnotationProperty .


###  http://www.w3.org/2004/02/skos/core#definition
<http://www.w3.org/2004/02/skos/core#definition> rdf:type owl:AnnotationProperty .


#################################################################
#    Object Properties
#################################################################

###  http://www.w3.org/2000/01/rdf-schema#seeAlso
rdfs:seeAlso rdf:type owl:ObjectProperty .


###  https://w3id.org/np/o/ntemplate/hasDefaultProvenance
<https://w3id.org/np/o/ntemplate/hasDefaultProvenance> rdf:type owl:ObjectProperty ;
                                                       rdfs:domain <https://w3id.org/np/o/ntemplate/AssertionTemplate> ;
                                                       rdfs:range <https://w3id.org/np/o/ntemplate/ProvenanceTemplate> ;
                                                       rdfs:isDefinedBy <https://w3id.org/np/o/ntemplate/latest/hasDefaultProvenance> ;
                                                       rdfs:label "has default provenance"@en ;
                                                       <http://www.w3.org/2004/02/skos/core#definition> "Indicates the default provenance template for a given assertion template."@en .


###  https://w3id.org/np/o/ntemplate/hasRequiredPubinfoElement
<https://w3id.org/np/o/ntemplate/hasRequiredPubinfoElement> rdf:type owl:ObjectProperty ;
                                                            rdfs:domain <https://w3id.org/np/o/ntemplate/AssertionTemplate> ;
                                                            rdfs:range <https://w3id.org/np/o/ntemplate/PubinfoTemplate> ;
                                                            rdfs:isDefinedBy <https://w3id.org/np/o/ntemplate/latest/hasRequiredPubinfoElement> ;
                                                            rdfs:label "has required publication info element"@en ;
                                                            <http://www.w3.org/2004/02/skos/core#definition> "Indicates the template of a required publication info element for a given assertion template."@en .


###  https://w3id.org/np/o/ntemplate/hasStatement
<https://w3id.org/np/o/ntemplate/hasStatement> rdf:type owl:ObjectProperty ;
                                               rdfs:range <https://w3id.org/np/o/ntemplate/TemplateStatement> ;
                                               rdfs:isDefinedBy <https://w3id.org/np/o/ntemplate/latest/hasStatement> ;
                                               rdfs:label "has statement"@en ;
                                               <http://www.w3.org/2004/02/skos/core#definition> "Connects an assertion template or a statement group within an assertion template to its included statements."@en .


###  https://w3id.org/np/o/ntemplate/possibleValue
<https://w3id.org/np/o/ntemplate/possibleValue> rdf:type owl:ObjectProperty ;
                                                rdfs:domain <https://w3id.org/np/o/ntemplate/UriPlaceholder> ;
                                                rdfs:isDefinedBy <https://w3id.org/np/o/ntemplate/latest/possibleValue> ;
                                                rdfs:label "possible value"@en ;
                                                <http://www.w3.org/2004/02/skos/core#definition> "Indicates a possible value for a restricted-choice or guided-choice placeholder."@en .


###  https://w3id.org/np/o/ntemplate/possibleValuesFrom
<https://w3id.org/np/o/ntemplate/possibleValuesFrom> rdf:type owl:ObjectProperty ;
                                                     rdfs:domain <https://w3id.org/np/o/ntemplate/UriPlaceholder> ;
                                                     rdfs:range <http://www.nanopub.org/nschema#Nanopublication> ;
                                                     rdfs:isDefinedBy <https://w3id.org/np/o/ntemplate/latest/possibleValuesFrom> ;
                                                     rdfs:label "possible values from"@en ;
                                                     <http://www.w3.org/2004/02/skos/core#definition> "Points to a nanopublication with possible values for a given restricted-choice or guided-choice placeholder."@en .


###  https://w3id.org/np/o/ntemplate/wasCreatedFromProvenanceTemplate
<https://w3id.org/np/o/ntemplate/wasCreatedFromProvenanceTemplate> rdf:type owl:ObjectProperty ;
                                                                   rdfs:domain <http://www.nanopub.org/nschema#Nanopublication> ;
                                                                   rdfs:range <https://w3id.org/np/o/ntemplate/ProvenanceTemplate> ;
                                                                   rdfs:isDefinedBy <https://w3id.org/np/o/ntemplate/latest/wasCreatedFromProvenanceTemplate> ;
                                                                   rdfs:label "was created from provenance template"@en ;
                                                                   <http://www.w3.org/2004/02/skos/core#definition> "Denotes that a nanopublication was created from the given provenance template."@en .


###  https://w3id.org/np/o/ntemplate/wasCreatedFromPubinfoTemplate
<https://w3id.org/np/o/ntemplate/wasCreatedFromPubinfoTemplate> rdf:type owl:ObjectProperty ;
                                                                rdfs:domain <http://www.nanopub.org/nschema#Nanopublication> ;
                                                                rdfs:range <https://w3id.org/np/o/ntemplate/PubinfoTemplate> ;
                                                                rdfs:isDefinedBy <https://w3id.org/np/o/ntemplate/latest/wasCreatedFromPubinfoTemplate> ;
                                                                rdfs:label "was created from publication info template"@en ;
                                                                <http://www.w3.org/2004/02/skos/core#definition> "Denotes that a nanopublication was created from the given publication info template."@en .


###  https://w3id.org/np/o/ntemplate/wasCreatedFromTemplate
<https://w3id.org/np/o/ntemplate/wasCreatedFromTemplate> rdf:type owl:ObjectProperty ;
                                                         rdfs:domain <http://www.nanopub.org/nschema#Nanopublication> ;
                                                         rdfs:range <https://w3id.org/np/o/ntemplate/AssertionTemplate> ;
                                                         rdfs:isDefinedBy <https://w3id.org/np/o/ntemplate/latest/wasCreatedFromTemplate> ;
                                                         rdfs:label "was created from template"@en ;
                                                         <http://www.w3.org/2004/02/skos/core#definition> "Denotes that a nanopublication was created from the given assertion template."@en .


#################################################################
#    Data properties
#################################################################

###  https://w3id.org/np/o/ntemplate/hasPrefix
<https://w3id.org/np/o/ntemplate/hasPrefix> rdf:type owl:DatatypeProperty ;
                                            rdfs:domain <https://w3id.org/np/o/ntemplate/UriPlaceholder> ;
                                            rdfs:isDefinedBy <https://w3id.org/np/o/ntemplate/latest/hasPrefix> ;
                                            rdfs:label "has prefix"@en ;
                                            <http://www.w3.org/2004/02/skos/core#definition> "Specifies a necessary URI prefix for a URI placeholder."@en .


###  https://w3id.org/np/o/ntemplate/hasPrefixLabel
<https://w3id.org/np/o/ntemplate/hasPrefixLabel> rdf:type owl:DatatypeProperty ;
                                                 rdfs:domain <https://w3id.org/np/o/ntemplate/UriPlaceholder> ;
                                                 rdfs:isDefinedBy <https://w3id.org/np/o/ntemplate/latest/hasPrefixLabel> ;
                                                 rdfs:label "has prefix label"@en ;
                                                 <http://www.w3.org/2004/02/skos/core#definition> "Specifies a label for the prefix part of a URI to be shown in the user interface."@en .


###  https://w3id.org/np/o/ntemplate/hasRegex
<https://w3id.org/np/o/ntemplate/hasRegex> rdf:type owl:DatatypeProperty ;
                                           rdfs:domain <https://w3id.org/np/o/ntemplate/Placeholder> ;
                                           rdfs:isDefinedBy <https://w3id.org/np/o/ntemplate/latest/hasRegex> ;
                                           rdfs:label "has regular expression"@en ;
                                           <http://www.w3.org/2004/02/skos/core#definition> "Specifies a regular expression pattern restricting the possible values for the given placeholder."@en .


###  https://w3id.org/np/o/ntemplate/hasTag
<https://w3id.org/np/o/ntemplate/hasTag> rdf:type owl:DatatypeProperty ;
                                         rdfs:domain <https://w3id.org/np/o/ntemplate/NanopubTemplate> ;
                                         rdfs:isDefinedBy <https://w3id.org/np/o/ntemplate/latest/hasTag> ;
                                         rdfs:label "has tag"@en ;
                                         <http://www.w3.org/2004/02/skos/core#definition> "Specifies a tag string that is used to group the templates in a user interface."@en .


###  https://w3id.org/np/o/ntemplate/possibleValuesFromApi
<https://w3id.org/np/o/ntemplate/possibleValuesFromApi> rdf:type owl:DatatypeProperty ;
                                                        rdfs:domain <https://w3id.org/np/o/ntemplate/GuidedChoicePlaceholder> ;
                                                        rdfs:isDefinedBy <https://w3id.org/np/o/ntemplate/latest/possibleValuesFromApi> ;
                                                        rdfs:label "possible values from API"@en ;
                                                        <http://www.w3.org/2004/02/skos/core#definition> "Specifies a URL pattern for an API to search for possible values for a guided-choice placeholder."@en .


###  https://w3id.org/np/o/ntemplate/statementOrder
<https://w3id.org/np/o/ntemplate/statementOrder> rdf:type owl:DatatypeProperty ;
                                                 rdfs:domain <https://w3id.org/np/o/ntemplate/NanopubTemplate> ;
                                                 rdfs:isDefinedBy <https://w3id.org/np/o/ntemplate/latest/statementOrder> ;
                                                 rdfs:label "statement order"@en ;
                                                 <http://www.w3.org/2004/02/skos/core#definition> "Specifies an integer value that defines the order in which statements appear."@en .


#################################################################
#    Classes
#################################################################

###  http://www.nanopub.org/nschema#Nanopublication
<http://www.nanopub.org/nschema#Nanopublication> rdf:type owl:Class ;
                                                 rdfs:label "Nanopublication" .


###  http://www.w3.org/1999/02/22-rdf-syntax-ns#Statement
rdf:Statement rdf:type owl:Class ;
              rdfs:subClassOf <https://w3id.org/np/o/ntemplate/TemplateStatement> .


###  https://w3id.org/np/o/ntemplate/AssertionTemplate
<https://w3id.org/np/o/ntemplate/AssertionTemplate> rdf:type owl:Class ;
                                                    rdfs:subClassOf <https://w3id.org/np/o/ntemplate/NanopubTemplate> ;
                                                    rdfs:isDefinedBy <https://w3id.org/np/o/ntemplate/latest/AssertionTemplate> ;
                                                    rdfs:label "Assertion Template"@en ;
                                                    <http://www.w3.org/2004/02/skos/core#definition> "A template that describes the assertion of a nanopublication."@en .


###  https://w3id.org/np/o/ntemplate/GroupedStatement
<https://w3id.org/np/o/ntemplate/GroupedStatement> rdf:type owl:Class ;
                                                   rdfs:subClassOf <https://w3id.org/np/o/ntemplate/TemplateStatement> ;
                                                   rdfs:isDefinedBy <https://w3id.org/np/o/ntemplate/latest/GroupedStatement> ;
                                                   rdfs:label "Grouped Statement"@en ;
                                                   <http://www.w3.org/2004/02/skos/core#definition> "A statement that grouped and thereby includes several simple statements."@en .


###  https://w3id.org/np/o/ntemplate/GuidedChoicePlaceholder
<https://w3id.org/np/o/ntemplate/GuidedChoicePlaceholder> rdf:type owl:Class ;
                                                          rdfs:subClassOf <https://w3id.org/np/o/ntemplate/UriPlaceholder> ;
                                                          rdfs:isDefinedBy <https://w3id.org/np/o/ntemplate/latest/GuidedChoicePlaceholder> ;
                                                          rdfs:label "Guided-Choice Placeholder"@en ;
                                                          <http://www.w3.org/2004/02/skos/core#definition> "A placeholder that stands for any URI (of a possible restricted set) and that comes with API-supported guidance on finding suitable URIs."@en .


###  https://w3id.org/np/o/ntemplate/IntroducedResource
<https://w3id.org/np/o/ntemplate/IntroducedResource> rdf:type owl:Class ;
                                                     rdfs:subClassOf <https://w3id.org/np/o/ntemplate/LocalResource> ;
                                                     rdfs:isDefinedBy <https://w3id.org/np/o/ntemplate/latest/IntroducedResource> ;
                                                     rdfs:label "Introduced Resource"@en ;
                                                     <http://www.w3.org/2004/02/skos/core#definition> "A resource in a template that represents a thing that is introduced (i.e. is referenced with 'npx:introduces' in the publication info of the nanopublications created from the template)."@en .


###  https://w3id.org/np/o/ntemplate/LiteralPlaceholder
<https://w3id.org/np/o/ntemplate/LiteralPlaceholder> rdf:type owl:Class ;
                                                     rdfs:subClassOf <https://w3id.org/np/o/ntemplate/ValuePlaceholder> ;
                                                     rdfs:isDefinedBy <https://w3id.org/np/o/ntemplate/latest/LiteralPlaceholder> ;
                                                     rdfs:label "Literal Placeholder"@en ;
                                                     <http://www.w3.org/2004/02/skos/core#definition> "A placeholder that stands for any RDF literal (of a possibly restricted set of possible literals)."@en .


###  https://w3id.org/np/o/ntemplate/LocalResource
<https://w3id.org/np/o/ntemplate/LocalResource> rdf:type owl:Class ;
                                                rdfs:isDefinedBy <https://w3id.org/np/o/ntemplate/latest/LocalResource> ;
                                                rdfs:label "Local Resource"@en ;
                                                <http://www.w3.org/2004/02/skos/core#definition> "A resource in a template that represents a local identifier to be minted."@en .


###  https://w3id.org/np/o/ntemplate/LongLiteralPlaceholder
<https://w3id.org/np/o/ntemplate/LongLiteralPlaceholder> rdf:type owl:Class ;
                                                         rdfs:subClassOf <https://w3id.org/np/o/ntemplate/LiteralPlaceholder> ;
                                                         rdfs:isDefinedBy <https://w3id.org/np/o/ntemplate/latest/LongLiteralPlaceholder> ;
                                                         rdfs:label "Long Literal Placeholder"@en ;
                                                         <http://www.w3.org/2004/02/skos/core#definition> "A placeholder that stands for an RDF literal that is expected to have a long value such that a bigger text field is convenient."@en .


###  https://w3id.org/np/o/ntemplate/NanopubTemplate
<https://w3id.org/np/o/ntemplate/NanopubTemplate> rdf:type owl:Class ;
                                                  rdfs:isDefinedBy <https://w3id.org/np/o/ntemplate/latest/NanopubTemplate> ;
                                                  rdfs:label "Nanopublication Template"@en ;
                                                  <http://www.w3.org/2004/02/skos/core#definition> "A template that describes a part of a nanopublication."@en .


###  https://w3id.org/np/o/ntemplate/OptionalStatement
<https://w3id.org/np/o/ntemplate/OptionalStatement> rdf:type owl:Class ;
                                                    rdfs:subClassOf <https://w3id.org/np/o/ntemplate/TemplateStatement> ;
                                                    rdfs:isDefinedBy <https://w3id.org/np/o/ntemplate/latest/OptionalStatement> ;
                                                    rdfs:label "Optional Statement"@en ;
                                                    <http://www.w3.org/2004/02/skos/core#definition> "A statement that is optional."@en .


###  https://w3id.org/np/o/ntemplate/Placeholder
<https://w3id.org/np/o/ntemplate/Placeholder> rdf:type owl:Class ;
                                              rdfs:isDefinedBy <https://w3id.org/np/o/ntemplate/latest/Placeholder> ;
                                              rdfs:label "Placeholder"@en ;
                                              <http://www.w3.org/2004/02/skos/core#definition> "A placeholder corresponding to an input component like a text field in a template."@en .


###  https://w3id.org/np/o/ntemplate/ProvenanceTemplate
<https://w3id.org/np/o/ntemplate/ProvenanceTemplate> rdf:type owl:Class ;
                                                     rdfs:subClassOf <https://w3id.org/np/o/ntemplate/NanopubTemplate> ;
                                                     rdfs:isDefinedBy <https://w3id.org/np/o/ntemplate/latest/ProvenanceTemplate> ;
                                                     rdfs:label "Provenance Template"@en ;
                                                     <http://www.w3.org/2004/02/skos/core#definition> "A template that describes the provenance of a nanopublication."@en .


###  https://w3id.org/np/o/ntemplate/PubinfoTemplate
<https://w3id.org/np/o/ntemplate/PubinfoTemplate> rdf:type owl:Class ;
                                                  rdfs:subClassOf <https://w3id.org/np/o/ntemplate/NanopubTemplate> ;
                                                  rdfs:isDefinedBy <https://w3id.org/np/o/ntemplate/latest/PubinfoTemplate> ;
                                                  rdfs:label "Publication Info Template"@en ;
                                                  <http://www.w3.org/2004/02/skos/core#definition> "A template that describes the publication info of a nanopublication."@en .


###  https://w3id.org/np/o/ntemplate/RepeatableStatement
<https://w3id.org/np/o/ntemplate/RepeatableStatement> rdf:type owl:Class ;
                                                      rdfs:subClassOf <https://w3id.org/np/o/ntemplate/TemplateStatement> ;
                                                      rdfs:isDefinedBy <https://w3id.org/np/o/ntemplate/latest/RepeatableStatement> ;
                                                      rdfs:label "Repeatable Statement"@en ;
                                                      <http://www.w3.org/2004/02/skos/core#definition> "A statement that can be repeated several times when the template is used."@en .


###  https://w3id.org/np/o/ntemplate/RestrictedChoicePlaceholder
<https://w3id.org/np/o/ntemplate/RestrictedChoicePlaceholder> rdf:type owl:Class ;
                                                              rdfs:subClassOf <https://w3id.org/np/o/ntemplate/UriPlaceholder> ;
                                                              rdfs:isDefinedBy <https://w3id.org/np/o/ntemplate/latest/RestrictedChoicePlaceholder> ;
                                                              rdfs:label "Restricted-Choice Placeholder"@en ;
                                                              <http://www.w3.org/2004/02/skos/core#definition> "A placeholder that stands for any URI of a pre-defined set of possible values."@en .


###  https://w3id.org/np/o/ntemplate/TemplateStatement
<https://w3id.org/np/o/ntemplate/TemplateStatement> rdf:type owl:Class ;
                                                    rdfs:isDefinedBy <https://w3id.org/np/o/ntemplate/latest/TemplateStatement> ;
                                                    rdfs:label "Template Statement"@en ;
                                                    <http://www.w3.org/2004/02/skos/core#definition> "A statement (simple or grouped) that is part of a template."@en .


###  https://w3id.org/np/o/ntemplate/TrustyUriPlaceholder
<https://w3id.org/np/o/ntemplate/TrustyUriPlaceholder> rdf:type owl:Class ;
                                                       rdfs:subClassOf <https://w3id.org/np/o/ntemplate/UriPlaceholder> ;
                                                       rdfs:isDefinedBy <https://w3id.org/np/o/ntemplate/latest/TrustyUriPlaceholder> ;
                                                       rdfs:label "Trusty URI Placeholder"@en ;
                                                       <http://www.w3.org/2004/02/skos/core#definition> "A placeholder that stands for any trusty URI (of a possibly restricted set)."@en .


###  https://w3id.org/np/o/ntemplate/UnlistedTemplate
<https://w3id.org/np/o/ntemplate/UnlistedTemplate> rdf:type owl:Class ;
                                                   rdfs:subClassOf <https://w3id.org/np/o/ntemplate/NanopubTemplate> ;
                                                   rdfs:isDefinedBy <https://w3id.org/np/o/ntemplate/latest/UnlistedTemplate> ;
                                                   rdfs:label "Unlisted Template"@en ;
                                                   <http://www.w3.org/2004/02/skos/core#definition> "A nanopublication template that is intended not to show up in template listings (but only to be used when explicitly referenced)."@en .


###  https://w3id.org/np/o/ntemplate/UriPlaceholder
<https://w3id.org/np/o/ntemplate/UriPlaceholder> rdf:type owl:Class ;
                                                 rdfs:subClassOf <https://w3id.org/np/o/ntemplate/ValuePlaceholder> ;
                                                 rdfs:isDefinedBy <https://w3id.org/np/o/ntemplate/latest/UriPlaceholder> ;
                                                 rdfs:label "URI Placeholder"@en ;
                                                 <http://www.w3.org/2004/02/skos/core#definition> "A placeholder that stands for any URI (of a possibly restricted set of URIs)."@en .


###  https://w3id.org/np/o/ntemplate/ValuePlaceholder
<https://w3id.org/np/o/ntemplate/ValuePlaceholder> rdf:type owl:Class ;
                                                   rdfs:subClassOf <https://w3id.org/np/o/ntemplate/Placeholder> ;
                                                   rdfs:isDefinedBy <https://w3id.org/np/o/ntemplate/latest/ValuePlaceholder> ;
                                                   rdfs:label "Value Placeholder"@en ;
                                                   <http://www.w3.org/2004/02/skos/core#definition> "A placeholder that stands for any RDF value (of a possibly restricted set of values), including URIs and literals."@en .


#################################################################
#    Individuals
#################################################################

###  https://w3id.org/np/o/ntemplate/ASSERTION
<https://w3id.org/np/o/ntemplate/ASSERTION> rdf:type owl:NamedIndividual ;
                                            rdfs:isDefinedBy <https://w3id.org/np/o/ntemplate/latest/ASSERTION> ;
                                            rdfs:label "ASSERTION"@en ;
                                            <http://www.w3.org/2004/02/skos/core#definition> "This is a template reference to the assertion of the nanopublication to be created."@en .


###  https://w3id.org/np/o/ntemplate/CREATOR
<https://w3id.org/np/o/ntemplate/CREATOR> rdf:type owl:NamedIndividual ;
                                          rdfs:isDefinedBy <https://w3id.org/np/o/ntemplate/latest/CREATOR> ;
                                          rdfs:label "CREATOR"@en ;
                                          <http://www.w3.org/2004/02/skos/core#definition> "This is a template reference to the creator of the nanopublication."@en .


###  https://w3id.org/np/o/ntemplate/NANOPUB
<https://w3id.org/np/o/ntemplate/NANOPUB> rdf:type owl:NamedIndividual ;
                                          rdfs:isDefinedBy <https://w3id.org/np/o/ntemplate/latest/NANOPUB> ;
                                          rdfs:label "NANOPUB"@en ;
                                          <http://www.w3.org/2004/02/skos/core#definition> "This is a template reference to the nanopublication to be created."@en .


###  Generated by the OWL API (version 5.1.11) https://github.com/owlcs/owlapi/
