<?xml version="1.0" encoding="utf-8"?>
<rdf:RDF
  xmlns:dcterms="http://purl.org/dc/terms/"
  xmlns:owl="http://www.w3.org/2002/07/owl#"
  xmlns:rdfs="http://www.w3.org/2000/01/rdf-schema#"
  xmlns:vann="http://purl.org/vocab/vann/"
  xmlns:rdf="http://www.w3.org/1999/02/22-rdf-syntax-ns#"
  xmlns:skos="http://www.w3.org/2004/02/skos/core#"
>
  <owl:AnnotationProperty rdf:about="http://purl.org/dc/terms/description"/>
  <owl:ObjectProperty rdf:about="https://w3id.org/np/o/ntemplate/wasCreatedFromProvenanceTemplate">
    <rdfs:domain rdf:resource="http://www.nanopub.org/nschema#Nanopublication"/>
    <rdfs:range rdf:resource="https://w3id.org/np/o/ntemplate/ProvenanceTemplate"/>
    <rdfs:isDefinedBy rdf:resource="https://w3id.org/np/o/ntemplate/latest/wasCreatedFromProvenanceTemplate"/>
    <rdfs:label xml:lang="en">was created from provenance template</rdfs:label>
    <skos:definition xml:lang="en">Denotes that a nanopublication was created from the given provenance template.</skos:definition>
  </owl:ObjectProperty>
  <owl:AnnotationProperty rdf:about="http://purl.org/dc/terms/license"/>
  <owl:Ontology rdf:about="https://w3id.org/np/o/ntemplate/NanopubTemplateOntology">
    <dcterms:creator rdf:resource="https://orcid.org/0000-0002-1267-0234"/>
    <dcterms:description>This is an ontology to describe nanopublication templates, which can be published as nanopublications themselves.</dcterms:description>
    <dcterms:license rdf:resource="https://creativecommons.org/publicdomain/zero/1.0/"/>
    <dcterms:title>Nanopublication Template Ontology</dcterms:title>
    <vann:preferredNamespacePrefix>nt</vann:preferredNamespacePrefix>
    <vann:preferredNamespaceUri>https://w3id.org/np/o/ntemplate/</vann:preferredNamespaceUri>
    <rdfs:isDefinedBy rdf:resource="https://w3id.org/np/o/ntemplate/latest/NanopubTemplateOntology"/>
  </owl:Ontology>
  <owl:Class rdf:about="https://w3id.org/np/o/ntemplate/TrustyUriPlaceholder">
    <rdfs:subClassOf rdf:resource="https://w3id.org/np/o/ntemplate/UriPlaceholder"/>
    <rdfs:isDefinedBy rdf:resource="https://w3id.org/np/o/ntemplate/latest/TrustyUriPlaceholder"/>
    <rdfs:label xml:lang="en">Trusty URI Placeholder</rdfs:label>
    <skos:definition xml:lang="en">A placeholder that stands for any trusty URI (of a possibly restricted set).</skos:definition>
  </owl:Class>
  <owl:DatatypeProperty rdf:about="https://w3id.org/np/o/ntemplate/possibleValuesFromApi">
    <rdfs:domain rdf:resource="https://w3id.org/np/o/ntemplate/GuidedChoicePlaceholder"/>
    <rdfs:isDefinedBy rdf:resource="https://w3id.org/np/o/ntemplate/latest/possibleValuesFromApi"/>
    <rdfs:label xml:lang="en">possible values from API</rdfs:label>
    <skos:definition xml:lang="en">Specifies a URL pattern for an API to search for possible values for a guided-choice placeholder.</skos:definition>
  </owl:DatatypeProperty>
  <owl:AnnotationProperty rdf:about="http://www.w3.org/2004/02/skos/core#definition"/>
  <owl:ObjectProperty rdf:about="https://w3id.org/np/o/ntemplate/hasRequiredPubinfoElement">
    <rdfs:domain rdf:resource="https://w3id.org/np/o/ntemplate/AssertionTemplate"/>
    <rdfs:range rdf:resource="https://w3id.org/np/o/ntemplate/PubinfoTemplate"/>
    <rdfs:isDefinedBy rdf:resource="https://w3id.org/np/o/ntemplate/latest/hasRequiredPubinfoElement"/>
    <rdfs:label xml:lang="en">has required publication info element</rdfs:label>
    <skos:definition xml:lang="en">Indicates the template of a required publication info element for a given assertion template.</skos:definition>
  </owl:ObjectProperty>
  <owl:ObjectProperty rdf:about="https://w3id.org/np/o/ntemplate/possibleValue">
    <rdfs:domain rdf:resource="https://w3id.org/np/o/ntemplate/UriPlaceholder"/>
    <rdfs:isDefinedBy rdf:resource="https://w3id.org/np/o/ntemplate/latest/possibleValue"/>
    <rdfs:label xml:lang="en">possible value</rdfs:label>
    <skos:definition xml:lang="en">Indicates a possible value for a restricted-choice or guided-choice placeholder.</skos:definition>
  </owl:ObjectProperty>
  <owl:ObjectProperty rdf:about="https://w3id.org/np/o/ntemplate/hasStatement">
    <rdfs:range rdf:resource="https://w3id.org/np/o/ntemplate/TemplateStatement"/>
    <rdfs:isDefinedBy rdf:resource="https://w3id.org/np/o/ntemplate/latest/hasStatement"/>
    <rdfs:label xml:lang="en">has statement</rdfs:label>
    <skos:definition xml:lang="en">Connects an assertion template or a statement group within an assertion template to its included statements.</skos:definition>
  </owl:ObjectProperty>
  <owl:AnnotationProperty rdf:about="http://purl.org/dc/terms/creator"/>
  <owl:DatatypeProperty rdf:about="https://w3id.org/np/o/ntemplate/hasPrefix">
    <rdfs:domain rdf:resource="https://w3id.org/np/o/ntemplate/UriPlaceholder"/>
    <rdfs:isDefinedBy rdf:resource="https://w3id.org/np/o/ntemplate/latest/hasPrefix"/>
    <rdfs:label xml:lang="en">has prefix</rdfs:label>
    <skos:definition xml:lang="en">Specifies a necessary URI prefix for a URI placeholder.</skos:definition>
  </owl:DatatypeProperty>
  <owl:Class rdf:about="https://w3id.org/np/o/ntemplate/IntroducedResource">
    <rdfs:subClassOf rdf:resource="https://w3id.org/np/o/ntemplate/LocalResource"/>
    <rdfs:isDefinedBy rdf:resource="https://w3id.org/np/o/ntemplate/latest/IntroducedResource"/>
    <rdfs:label xml:lang="en">Introduced Resource</rdfs:label>
    <skos:definition xml:lang="en">A resource in a template that represents a thing that is introduced (i.e. is referenced with 'npx:introduces' in the publication info of the nanopublications created from the template).</skos:definition>
  </owl:Class>
  <owl:NamedIndividual rdf:about="https://w3id.org/np/o/ntemplate/ASSERTION">
    <rdfs:isDefinedBy rdf:resource="https://w3id.org/np/o/ntemplate/latest/ASSERTION"/>
    <rdfs:label xml:lang="en">ASSERTION</rdfs:label>
    <skos:definition xml:lang="en">This is a template reference to the assertion of the nanopublication to be created.</skos:definition>
  </owl:NamedIndividual>
  <owl:Class rdf:about="http://www.w3.org/1999/02/22-rdf-syntax-ns#Statement">
    <rdfs:subClassOf rdf:resource="https://w3id.org/np/o/ntemplate/TemplateStatement"/>
  </owl:Class>
  <owl:NamedIndividual rdf:about="https://w3id.org/np/o/ntemplate/CREATOR">
    <rdfs:isDefinedBy rdf:resource="https://w3id.org/np/o/ntemplate/latest/CREATOR"/>
    <rdfs:label xml:lang="en">CREATOR</rdfs:label>
    <skos:definition xml:lang="en">This is a template reference to the creator of the nanopublication.</skos:definition>
  </owl:NamedIndividual>
  <owl:ObjectProperty rdf:about="https://w3id.org/np/o/ntemplate/wasCreatedFromPubinfoTemplate">
    <rdfs:domain rdf:resource="http://www.nanopub.org/nschema#Nanopublication"/>
    <rdfs:range rdf:resource="https://w3id.org/np/o/ntemplate/PubinfoTemplate"/>
    <rdfs:isDefinedBy rdf:resource="https://w3id.org/np/o/ntemplate/latest/wasCreatedFromPubinfoTemplate"/>
    <rdfs:label xml:lang="en">was created from publication info template</rdfs:label>
    <skos:definition xml:lang="en">Denotes that a nanopublication was created from the given publication info template.</skos:definition>
  </owl:ObjectProperty>
  <owl:Class rdf:about="https://w3id.org/np/o/ntemplate/UnlistedTemplate">
    <rdfs:subClassOf rdf:resource="https://w3id.org/np/o/ntemplate/NanopubTemplate"/>
    <rdfs:isDefinedBy rdf:resource="https://w3id.org/np/o/ntemplate/latest/UnlistedTemplate"/>
    <rdfs:label xml:lang="en">Unlisted Template</rdfs:label>
    <skos:definition xml:lang="en">A nanopublication template that is intended not to show up in template listings (but only to be used when explicitly referenced).</skos:definition>
  </owl:Class>
  <owl:Class rdf:about="https://w3id.org/np/o/ntemplate/GroupedStatement">
    <rdfs:subClassOf rdf:resource="https://w3id.org/np/o/ntemplate/TemplateStatement"/>
    <rdfs:isDefinedBy rdf:resource="https://w3id.org/np/o/ntemplate/latest/GroupedStatement"/>
    <rdfs:label xml:lang="en">Grouped Statement</rdfs:label>
    <skos:definition xml:lang="en">A statement that grouped and thereby includes several simple statements.</skos:definition>
  </owl:Class>
  <owl:ObjectProperty rdf:about="https://w3id.org/np/o/ntemplate/wasCreatedFromTemplate">
    <rdfs:domain rdf:resource="http://www.nanopub.org/nschema#Nanopublication"/>
    <rdfs:range rdf:resource="https://w3id.org/np/o/ntemplate/AssertionTemplate"/>
    <rdfs:isDefinedBy rdf:resource="https://w3id.org/np/o/ntemplate/latest/wasCreatedFromTemplate"/>
    <rdfs:label xml:lang="en">was created from template</rdfs:label>
    <skos:definition xml:lang="en">Denotes that a nanopublication was created from the given assertion template.</skos:definition>
  </owl:ObjectProperty>
  <owl:ObjectProperty rdf:about="https://w3id.org/np/o/ntemplate/hasDefaultProvenance">
    <rdfs:domain rdf:resource="https://w3id.org/np/o/ntemplate/AssertionTemplate"/>
    <rdfs:range rdf:resource="https://w3id.org/np/o/ntemplate/ProvenanceTemplate"/>
    <rdfs:isDefinedBy rdf:resource="https://w3id.org/np/o/ntemplate/latest/hasDefaultProvenance"/>
    <rdfs:label xml:lang="en">has default provenance</rdfs:label>
    <skos:definition xml:lang="en">Indicates the default provenance template for a given assertion template.</skos:definition>
  </owl:ObjectProperty>
  <owl:DatatypeProperty rdf:about="https://w3id.org/np/o/ntemplate/hasRegex">
    <rdfs:domain rdf:resource="https://w3id.org/np/o/ntemplate/Placeholder"/>
    <rdfs:isDefinedBy rdf:resource="https://w3id.org/np/o/ntemplate/latest/hasRegex"/>
    <rdfs:label xml:lang="en">has regular expression</rdfs:label>
    <skos:definition xml:lang="en">Specifies a regular expression pattern restricting the possible values for the given placeholder.</skos:definition>
  </owl:DatatypeProperty>
  <owl:ObjectProperty rdf:about="https://w3id.org/np/o/ntemplate/possibleValuesFrom">
    <rdfs:domain rdf:resource="https://w3id.org/np/o/ntemplate/UriPlaceholder"/>
    <rdfs:range rdf:resource="http://www.nanopub.org/nschema#Nanopublication"/>
    <rdfs:isDefinedBy rdf:resource="https://w3id.org/np/o/ntemplate/latest/possibleValuesFrom"/>
    <rdfs:label xml:lang="en">possible values from</rdfs:label>
    <skos:definition xml:lang="en">Points to a nanopublication with possible values for a given restricted-choice or guided-choice placeholder.</skos:definition>
  </owl:ObjectProperty>
  <owl:Class rdf:about="https://w3id.org/np/o/ntemplate/RestrictedChoicePlaceholder">
    <rdfs:subClassOf rdf:resource="https://w3id.org/np/o/ntemplate/UriPlaceholder"/>
    <rdfs:isDefinedBy rdf:resource="https://w3id.org/np/o/ntemplate/latest/RestrictedChoicePlaceholder"/>
    <rdfs:label xml:lang="en">Restricted-Choice Placeholder</rdfs:label>
    <skos:definition xml:lang="en">A placeholder that stands for any URI of a pre-defined set of possible values.</skos:definition>
  </owl:Class>
  <owl:DatatypeProperty rdf:about="https://w3id.org/np/o/ntemplate/hasTag">
    <rdfs:domain rdf:resource="https://w3id.org/np/o/ntemplate/NanopubTemplate"/>
    <rdfs:isDefinedBy rdf:resource="https://w3id.org/np/o/ntemplate/latest/hasTag"/>
    <rdfs:label xml:lang="en">has tag</rdfs:label>
    <skos:definition xml:lang="en">Specifies a tag string that is used to group the templates in a user interface.</skos:definition>
  </owl:DatatypeProperty>
  <owl:NamedIndividual rdf:about="https://w3id.org/np/o/ntemplate/NANOPUB">
    <rdfs:isDefinedBy rdf:resource="https://w3id.org/np/o/ntemplate/latest/NANOPUB"/>
    <rdfs:label xml:lang="en">NANOPUB</rdfs:label>
    <skos:definition xml:lang="en">This is a template reference to the nanopublication to be created.</skos:definition>
  </owl:NamedIndividual>
  <owl:Class rdf:about="https://w3id.org/np/o/ntemplate/OptionalStatement">
    <rdfs:subClassOf rdf:resource="https://w3id.org/np/o/ntemplate/TemplateStatement"/>
    <rdfs:isDefinedBy rdf:resource="https://w3id.org/np/o/ntemplate/latest/OptionalStatement"/>
    <rdfs:label xml:lang="en">Optional Statement</rdfs:label>
    <skos:definition xml:lang="en">A statement that is optional.</skos:definition>
  </owl:Class>
  <owl:Class rdf:about="https://w3id.org/np/o/ntemplate/LongLiteralPlaceholder">
    <rdfs:subClassOf rdf:resource="https://w3id.org/np/o/ntemplate/LiteralPlaceholder"/>
    <rdfs:isDefinedBy rdf:resource="https://w3id.org/np/o/ntemplate/latest/LongLiteralPlaceholder"/>
    <rdfs:label xml:lang="en">Long Literal Placeholder</rdfs:label>
    <skos:definition xml:lang="en">A placeholder that stands for an RDF literal that is expected to have a long value such that a bigger text field is convenient.</skos:definition>
  </owl:Class>
  <owl:AnnotationProperty rdf:about="http://purl.org/vocab/vann/preferredNamespaceUri"/>
  <owl:Class rdf:about="https://w3id.org/np/o/ntemplate/RepeatableStatement">
    <rdfs:subClassOf rdf:resource="https://w3id.org/np/o/ntemplate/TemplateStatement"/>
    <rdfs:isDefinedBy rdf:resource="https://w3id.org/np/o/ntemplate/latest/RepeatableStatement"/>
    <rdfs:label xml:lang="en">Repeatable Statement</rdfs:label>
    <skos:definition xml:lang="en">A statement that can be repeated several times when the template is used.</skos:definition>
  </owl:Class>
  <owl:AnnotationProperty rdf:about="http://purl.org/dc/terms/title"/>
  <owl:DatatypeProperty rdf:about="https://w3id.org/np/o/ntemplate/statementOrder">
    <rdfs:domain rdf:resource="https://w3id.org/np/o/ntemplate/NanopubTemplate"/>
    <rdfs:isDefinedBy rdf:resource="https://w3id.org/np/o/ntemplate/latest/statementOrder"/>
    <rdfs:label xml:lang="en">statement order</rdfs:label>
    <skos:definition xml:lang="en">Specifies an integer value that defines the order in which statements appear.</skos:definition>
  </owl:DatatypeProperty>
  <owl:DatatypeProperty rdf:about="https://w3id.org/np/o/ntemplate/hasPrefixLabel">
    <rdfs:domain rdf:resource="https://w3id.org/np/o/ntemplate/UriPlaceholder"/>
    <rdfs:isDefinedBy rdf:resource="https://w3id.org/np/o/ntemplate/latest/hasPrefixLabel"/>
    <rdfs:label xml:lang="en">has prefix label</rdfs:label>
    <skos:definition xml:lang="en">Specifies a label for the prefix part of a URI to be shown in the user interface.</skos:definition>
  </owl:DatatypeProperty>
  <owl:AnnotationProperty rdf:about="http://purl.org/vocab/vann/preferredNamespacePrefix"/>
  <owl:ObjectProperty rdf:about="http://www.w3.org/2000/01/rdf-schema#seeAlso"/>
  <owl:Class rdf:about="https://w3id.org/np/o/ntemplate/ValuePlaceholder">
    <rdfs:subClassOf rdf:resource="https://w3id.org/np/o/ntemplate/Placeholder"/>
    <rdfs:isDefinedBy rdf:resource="https://w3id.org/np/o/ntemplate/latest/ValuePlaceholder"/>
    <rdfs:label xml:lang="en">Value Placeholder</rdfs:label>
    <skos:definition xml:lang="en">A placeholder that stands for any RDF value (of a possibly restricted set of values), including URIs and literals.</skos:definition>
  </owl:Class>
  <owl:Class rdf:about="https://w3id.org/np/o/ntemplate/GuidedChoicePlaceholder">
    <rdfs:subClassOf rdf:resource="https://w3id.org/np/o/ntemplate/UriPlaceholder"/>
    <rdfs:isDefinedBy rdf:resource="https://w3id.org/np/o/ntemplate/latest/GuidedChoicePlaceholder"/>
    <rdfs:label xml:lang="en">Guided-Choice Placeholder</rdfs:label>
    <skos:definition xml:lang="en">A placeholder that stands for any URI (of a possible restricted set) and that comes with API-supported guidance on finding suitable URIs.</skos:definition>
  </owl:Class>
  <owl:Class rdf:about="https://w3id.org/np/o/ntemplate/LocalResource">
    <rdfs:isDefinedBy rdf:resource="https://w3id.org/np/o/ntemplate/latest/LocalResource"/>
    <rdfs:label xml:lang="en">Local Resource</rdfs:label>
    <skos:definition xml:lang="en">A resource in a template that represents a local identifier to be minted.</skos:definition>
  </owl:Class>
  <owl:Class rdf:about="https://w3id.org/np/o/ntemplate/PubinfoTemplate">
    <rdfs:subClassOf rdf:resource="https://w3id.org/np/o/ntemplate/NanopubTemplate"/>
    <rdfs:isDefinedBy rdf:resource="https://w3id.org/np/o/ntemplate/latest/PubinfoTemplate"/>
    <rdfs:label xml:lang="en">Publication Info Template</rdfs:label>
    <skos:definition xml:lang="en">A template that describes the publication info of a nanopublication.</skos:definition>
  </owl:Class>
  <owl:Class rdf:about="https://w3id.org/np/o/ntemplate/TemplateStatement">
    <rdfs:isDefinedBy rdf:resource="https://w3id.org/np/o/ntemplate/latest/TemplateStatement"/>
    <rdfs:label xml:lang="en">Template Statement</rdfs:label>
    <skos:definition xml:lang="en">A statement (simple or grouped) that is part of a template.</skos:definition>
  </owl:Class>
  <owl:Class rdf:about="http://www.nanopub.org/nschema#Nanopublication">
    <rdfs:label>Nanopublication</rdfs:label>
  </owl:Class>
  <owl:Class rdf:about="https://w3id.org/np/o/ntemplate/UriPlaceholder">
    <rdfs:subClassOf rdf:resource="https://w3id.org/np/o/ntemplate/ValuePlaceholder"/>
    <rdfs:isDefinedBy rdf:resource="https://w3id.org/np/o/ntemplate/latest/UriPlaceholder"/>
    <rdfs:label xml:lang="en">URI Placeholder</rdfs:label>
    <skos:definition xml:lang="en">A placeholder that stands for any URI (of a possibly restricted set of URIs).</skos:definition>
  </owl:Class>
  <owl:Class rdf:about="https://w3id.org/np/o/ntemplate/AssertionTemplate">
    <rdfs:subClassOf rdf:resource="https://w3id.org/np/o/ntemplate/NanopubTemplate"/>
    <rdfs:isDefinedBy rdf:resource="https://w3id.org/np/o/ntemplate/latest/AssertionTemplate"/>
    <rdfs:label xml:lang="en">Assertion Template</rdfs:label>
    <skos:definition xml:lang="en">A template that describes the assertion of a nanopublication.</skos:definition>
  </owl:Class>
  <owl:Class rdf:about="https://w3id.org/np/o/ntemplate/ProvenanceTemplate">
    <rdfs:subClassOf rdf:resource="https://w3id.org/np/o/ntemplate/NanopubTemplate"/>
    <rdfs:isDefinedBy rdf:resource="https://w3id.org/np/o/ntemplate/latest/ProvenanceTemplate"/>
    <rdfs:label xml:lang="en">Provenance Template</rdfs:label>
    <skos:definition xml:lang="en">A template that describes the provenance of a nanopublication.</skos:definition>
  </owl:Class>
  <owl:Class rdf:about="https://w3id.org/np/o/ntemplate/NanopubTemplate">
    <rdfs:isDefinedBy rdf:resource="https://w3id.org/np/o/ntemplate/latest/NanopubTemplate"/>
    <rdfs:label xml:lang="en">Nanopublication Template</rdfs:label>
    <skos:definition xml:lang="en">A template that describes a part of a nanopublication.</skos:definition>
  </owl:Class>
  <owl:Class rdf:about="https://w3id.org/np/o/ntemplate/LiteralPlaceholder">
    <rdfs:subClassOf rdf:resource="https://w3id.org/np/o/ntemplate/ValuePlaceholder"/>
    <rdfs:isDefinedBy rdf:resource="https://w3id.org/np/o/ntemplate/latest/LiteralPlaceholder"/>
    <rdfs:label xml:lang="en">Literal Placeholder</rdfs:label>
    <skos:definition xml:lang="en">A placeholder that stands for any RDF literal (of a possibly restricted set of possible literals).</skos:definition>
  </owl:Class>
  <owl:Class rdf:about="https://w3id.org/np/o/ntemplate/Placeholder">
    <rdfs:isDefinedBy rdf:resource="https://w3id.org/np/o/ntemplate/latest/Placeholder"/>
    <rdfs:label xml:lang="en">Placeholder</rdfs:label>
    <skos:definition xml:lang="en">A placeholder corresponding to an input component like a text field in a template.</skos:definition>
  </owl:Class>
</rdf:RDF>
